## n!

$$ n! = ? $$

$$ n! = n(n - 1)(n - 2)... 1 $$

$$ \frac{d}{dx} x^n = n x^{n - 1} $$

$$ \frac{d^2}{dx^2} x^n = n(n - 1) x^{n - 2} $$

$$ \frac{d^a}{dx^a} x^n = \frac{n! x^{n - a}}{(n - a)!} $$

$$ \frac{d^n}{dx^n} x^n = \frac{n! x^{n - n}}{(n - n)!} = n! $$

$$ \frac{d^n}{dx^n} \frac{1}{x} = \frac{(-1)^n n!}{x^{n - 1}} $$

$$ \frac{d^n}{dx^n} (-\frac{1}{x}) = \frac{n!}{(-x)^{n + 1}} $$

$\quad$ $\quad$ $\quad$ $\quad$ $\quad$ $\quad$  if $\frac{n!}{(-x)^{n + 1}}$ is a function of x and x can be a constant then $\frac{d^n}{dx^n} (-\frac{1}{x})$ is not. so $\frac{n!}{(-x)^{n + 1}}$ at $x = -1$ is $n!$

$\quad$ $\quad$ $\quad$ $\quad$ $\quad$ $\quad$ $\quad$ $\quad$ $\quad$ $\quad$ $\quad$ $\quad$ $\quad$ problem solved!... but that is a bit too many derivitaves...
