## quadratic

$$ ax^2 + bx + c = (d) x^2 + (-d(s_1 + s_2)) x + (d s_1 s_2) = d(x - s_1)(x - s_2) $$

now, I will say that if these are equal, than they have the same terms, so I will use the first to simplify, the second to solve for $i$, and the third to solve for $k^2$ (I'll explain later)

$$ a = d $$

$$ x^2 + \frac{b}{a} x + \frac{c}{a} = (x - s_1)(x - s_2) = x^2 + (-(s_1 + s_2)) x + (s_1 s_2) $$

$$ s_1 = i + j $$

$$ s_2 = i - j $$

$$ as_1^2 + bs_1 + c = a(s_1 - s_1)(s_1 - s_2) = a0(s_1 - s_2) = 0 $$

$$ as_2^2 + bs_2 + c = a(s_2 - s_1)(s_2 - s_2) = a(s_2 - s_1)0 = 0 $$

$$ as_1^2 + bs_1 + c = 0 $$

$$ as_2^2 + bs_2 + c = 0 $$

$$ as^2 + bs + c = 0 $$

$$ s = i \pm j = i \pm \sqrt{j^2} = i + k $$

$$ k^2 = j^2 $$

$$ \frac{b}{a} = -(s_1 + s_2) $$

$$ \frac{b}{2a} = -\frac{s_1 + s_2}{2} $$

$$ -\frac{b}{2a} = \frac{s_1 + s_2}{2} = i $$

$$ i = -\frac{b}{2a} $$

$$ \frac{c}{a} = s_1 s_2 = (i + j)(i - j) = i^2 - j^2 = \frac{b^2}{4a^2} - j^2 $$

$$ j^2 = \frac{b^2}{4a^2} - \frac{c}{a} = \frac{b^2 - 4ac}{4a^2} $$

$$ s = k - \frac{b}{2a} $$

$$ k^2 = \frac{b^2 - 4ac}{4a^2} $$

$$ s = -\frac{b}{2a} \pm \sqrt{\frac{b^2 - 4ac}{4a^2}} $$
